Lp2lc/Active/STLC/__Infer_umbral.lean
@@ -13,8 +13,9 @@ namespace Umbral
 
 section variable [@ProvingBase F]
 
-structure InferenceWProof (trm: AST.Trm F) : Type where
-  typ: AST.Typ F
+structure InferenceWProof (trm2typ: AST.Trm2Typ F) : Type where
+  trm := trm2typ.trm
+  typ := trm2typ.typ
   sameInfer: trm.infer.isDecidable (λ t2 => typ <= t2)
   safetyProof: Safety trm typ
 
@@ -31,8 +32,7 @@ there is no guarantee that typeUID & valueUID will be identical, so this is the 
 
 class ProvingEnv where
   base: @ProvingBase F
-  proofGroup : FBound F.Index (AST.Trm F)
-  proofCtx : FBound.Aux proofGroup (@InferenceWProof F base) -- TODO: need a concrete value type to save proof
+  proofCtx : base.trm2typCtx.Aux (λ t => @InferenceWProof t) -- TODO: need a concrete value type to save proof
 
 instance [env: @ProvingEnv F] : @ProvingBase F := env.base
 
